Add soundness of StateT

Classes/SoundMonad.v
@@ -10,13 +10,13 @@ Section monad_sound.
   Context {M_galois : ∀ A A' : Type, Galois A A' → Galois (M A) (M' A')}.
 
   Class SoundMonad : Type := {
-    fmap_sound : ∀ {A A' B B' : Type} `{Galois A A', Galois B B'}, 
+    fmap_sound : ∀ (A A' B B' : Type) `{Galois A A', Galois B B'}, 
       gamma (B:=(A' → B') → M' A' → M' B') fmap fmap;
-    pure_sound : ∀ {A A': Type} `{Galois A A'},
+    pure_sound : ∀ (A A': Type) `{Galois A A'},
       gamma (B:= (A' → M' A')) pure pure;
-    app_sound : ∀ {A A' B B' : Type} `{Galois A A', Galois B B'}, 
+    app_sound : ∀ (A A' B B' : Type) `{Galois A A', Galois B B'}, 
       gamma (B:=M' (A' → B') → M' A' → M' B') app app;
-    bind_sound : ∀ {A A' B B' : Type} `{Galois A A', Galois B B'},
+    bind_sound : ∀ (A A' B B' : Type) `{Galois A A', Galois B B'},
       gamma (B:=M' A' → (A' → M' B') → M' B') bindM bindM;
   }.
 End monad_sound.
